{-# OPTIONS --lossy-unification #-}

open import Foundation.Essential
  hiding (_âˆˆ_) renaming (_âˆˆá´¸_ to _âˆˆ_)
open import Foundation.Data.Nat.AlternativeOrder

module Enumerability.ListView.Instance where
open import Enumerability.ListView.Base
open import Enumerability.ListView.Combine

private variable
  m n o : â„•

instance
  enumğ”¹ : Enum ğ”¹
  enumğ”¹ = mkEnum (Î» _ â†’ true âˆ· [ false ]) (Î» n â†’ [] , refl)
    Î» { true â†’  ex 0 $ here refl
      ; false â†’ ex 0 $ there (here refl) }

  enumâ„• : Enum â„•
  enumâ„• = mkEnum e c w where
    e : ğ•ƒâ‚™ â„•
    e zero = [ 0 ]
    e (suc n) = e n ++ [ suc n ]
    c : Cumulation e
    c _ = _ , refl
    w : âˆ€ n â†’ e witness n
    w n = ex n (H n) where
      H : âˆ€ n â†’ n âˆˆ e n
      H zero = here refl
      H (suc n) = âˆˆ-++âºÊ³ (here refl)

  enumÃ— : â¦ƒ Enum A â¦„ â†’ â¦ƒ Enum B â¦„ â†’ Enum (A Ã— B)
  enumÃ— {A} {B} = mkEnum e c w where
    e : ğ•ƒâ‚™ (A Ã— B)
    e zero = enum 0 [Ã—] enum 0
    e (suc n) = e n ++ enum n [Ã—] enum n
    c : Cumulation e
    c n = enum n [Ã—] enum n , refl
    w : âˆ€ xy â†’ e witness xy
    w (x , y) = ğŸ™.map2 H (wit x) (wit y) where
      H : Witness enum x â†’ Witness enum y â†’ Witness e (x , y)
      H (m , xâˆˆfm) (n , xâˆˆgn) = suc (m + n) , âˆˆ-++âºÊ³ H2 where
        H2 : (x , y) âˆˆ enum (m + n) [Ã—] enum (m + n)
        H2 = âˆˆ[Ã—]-intro (cum-â‰¤â†’âŠ† cum mâ‰¤m+n xâˆˆfm) (cum-â‰¤â†’âŠ† cum mâ‰¤n+m xâˆˆgn)

  enumVec : â¦ƒ Enum A â¦„ â†’ Enum (ğ• A n)
  enumVec {A} = mkEnum e c w where

    e : ğ•ƒâ‚™ (ğ• A n)
    e zero = []
    e {n} (suc m) = e m ++ combine (enum m) n

    c : Cumulation e
    c _ = _ , refl

    e-â‰¤â†’âŠ† : {xâƒ— : ğ• A n} â†’ m â‰¤ o â†’ xâƒ— âˆˆ e m â†’ xâƒ— âˆˆ combine (enum o) n
    e-â‰¤â†’âŠ† {m = suc m} smâ‰¤o H with âˆˆ-++â» (e m) H
    ... | injâ‚ xâƒ—âˆˆen   = e-â‰¤â†’âŠ† (m+nâ‰¤oâ‡’nâ‰¤o 1 smâ‰¤o) xâƒ—âˆˆen
    ... | injâ‚‚ xâƒ—âˆˆcomb = combine-â‰¤â†’âŠ† cum (m+nâ‰¤oâ‡’nâ‰¤o 1 smâ‰¤o) xâƒ—âˆˆcomb

    w : (xâƒ— : ğ• A n) â†’ e witness xâƒ—
    w [] = ex 1 (here refl)
    w (x âˆ· xâƒ—) = ğŸ™.map2 H (wit x) (w xâƒ—) where
      H : Witness enum x â†’ Witness e xâƒ— â†’ Witness e (x âˆ· xâƒ—)
      H (m , Hm) (suc n , Hn) = suc m + suc n , âˆˆ-++âºÊ³ (âˆˆmap[Ã—]-intro H1 H2) where
        H1 : x âˆˆ enum (m + suc n)
        H1 = cum-â‰¤â†’âŠ† cum mâ‰¤m+n Hm
        H2 : xâƒ— âˆˆ combine (enum (m + suc n)) _
        H2 = e-â‰¤â†’âŠ† mâ‰¤n+m Hn
