module Enumerability.View.Lists where

open import Foundation.Prelude
open import Foundation.Prop.Truncation
open import Foundation.Prop.Logic
open import Foundation.Prop.Iff

open import Foundation.Data.Nat
open import Foundation.Data.Nat.AlternativeOrder
open import Foundation.Data.Maybe
open import Foundation.Data.Sigma
open import Foundation.Data.Sum
open import Foundation.Data.List
open import Foundation.Data.List.SetTheoretic
open import Foundation.Data.List.Discrete (discreteÃ— discreteâ„• discreteâ„•)

open import Foundation.Relation.Nullary.Discrete
open import Foundation.Relation.Unary.Countable

import Enumerability.View.Maybe as â“‚

ğ•ƒâ‚™ : ğ•‹ â„“ â†’ ğ•‹ â„“
ğ•ƒâ‚™ A = â„• â†’ ğ•ƒ A

Cumulation : ğ•ƒâ‚™ A â†’ ğ•‹ _
Cumulation f = âˆ€ n â†’ Î£ xs ï¼Œ f (suc n) â‰¡ f n ++ xs

module _ {f : ğ•ƒâ‚™ A} (cum : Cumulation f) where

  cum-â‰¤â†’++ : {m n : â„•} â†’ m â‰¤ n â†’ Î£ xs ï¼Œ f n â‰¡ f m ++ xs
  cum-â‰¤â†’++ {m = n} {n} â‰¤-refl = [] , sym (++-identityÊ³ (f n))
  cum-â‰¤â†’++ {m} {suc n} (â‰¤-step mâ‰¤n) with cum n | cum-â‰¤â†’++ mâ‰¤n
  ... | xs , Hâ‚ | ys , Hâ‚‚ = (ys ++ xs) ,
    f (suc n)         â‰¡âŸ¨ Hâ‚ âŸ©
    f n ++ xs         â‰¡âŸ¨ cong (_++ xs) Hâ‚‚ âŸ©
    (f m ++ ys) ++ xs â‰¡âŸ¨ ++-assoc (f m) ys xs âŸ©
    f m ++ ys ++ xs   âˆ

  cum-â‰¤â†’âŠ† : {m n : â„•} â†’ m â‰¤ n â†’ f m âŠ† f n
  cum-â‰¤â†’âŠ† mâ‰¤n xâˆˆfm with cum-â‰¤â†’++ mâ‰¤n
  ... | xs , eq = subst (_ âˆˆ_) eq (âˆˆ-++âºË¡ xâˆˆfm)

Witness : ğ•ƒâ‚™ A â†’ A â†’ ğ•‹ _
Witness f x = Î£ n ï¼Œ x âˆˆ f n

_witness_ : ğ•ƒâ‚™ A â†’ A â†’ ğ•‹ _
f witness x = âˆ¥ Witness f x âˆ¥â‚

record Enum (A : ğ•‹ â„“) : ğ•‹ (â„“ âº) where
  constructor mkEnum
  field
    enum : ğ•ƒâ‚™ A
    cum : Cumulation enum
    wit : âˆ€ x â†’ enum witness x

record Enumâ„™ {A : ğ•‹ â„“} (P : A â†’ ğ•‹ â„“â€²) : ğ•‹ (â„“ âŠ” â„“â€²) where
  constructor mkEnumâ„™
  field
    enumâ„™ : ğ•ƒâ‚™ A
    cumâ„™ : Cumulation enumâ„™
    witâ„™ : âˆ€ x â†’ P x â†” enumâ„™ witness x

open Enum â¦ƒ...â¦„ public
open Enumâ„™ â¦ƒ...â¦„ public

Enumâ†”â„™ : Enum A â†” Enumâ„™ Î» (_ : A) â†’ âŠ¤
Enumâ†”â„™ = â‡’: (Î» (mkEnum f cum H) â†’ mkEnumâ„™ f cum Î» x â†’ â‡’: (Î» _ â†’ H x) â‡: (Î» _ â†’ tt))
          â‡: (Î» (mkEnumâ„™ f cum H) â†’ mkEnum f cum Î» x â†’ H x .â‡’ tt)

enumerable : ğ•‹ â„“ â†’ ğ•‹ _
enumerable A = âˆ¥ Enum A âˆ¥â‚

enumerableâ„™ : (A â†’ ğ•‹ â„“) â†’ ğ•‹ _
enumerableâ„™ P = âˆ¥ Enumâ„™ P âˆ¥â‚

enumerableâ†”â„™ : enumerable A â†” enumerableâ„™ Î» (_ : A) â†’ âŠ¤
enumerableâ†”â„™ = â†”-map Enumâ†”â„™

Enumğ”¹ : Enum ğ”¹
Enumğ”¹ = mkEnum (Î» _ â†’ true âˆ· [ false ]) (Î» n â†’ [] , refl)
  Î» { true â†’  ex 0 (here refl)
    ; false â†’ ex 0 (there $ here refl) }

eâ„• : ğ•ƒâ‚™ â„•
eâ„• zero = [ 0 ]
eâ„• (suc n) = eâ„• n ++ [ suc n ]

Enumâ„• : Enum â„•
Enumâ„• = mkEnum eâ„• (Î» n â†’ [ suc n ] , refl) Î» n â†’ ex n (H n) where
  H : âˆ€ n â†’ n âˆˆ eâ„• n
  H zero = here refl
  H (suc n) = âˆˆ-++âºÊ³ (here refl)

âˆˆeâ„•-intro : âˆ€ m n â†’ m â‰¤ n â†’ m âˆˆ eâ„• n
âˆˆeâ„•-intro zero zero â‰¤-refl = here refl
âˆˆeâ„•-intro (suc m) (suc m) â‰¤-refl = âˆˆ-++âºÊ³ (here refl)
âˆˆeâ„•-intro m (suc n) (â‰¤-step mâ‰¤n) = âˆˆ-++âºË¡ (âˆˆeâ„•-intro m n mâ‰¤n)

eâ„•-length : âˆ€ n â†’ length (eâ„• n) â‰¡ suc n
eâ„•-length zero = refl
eâ„•-length (suc n) =
  length (eâ„• (suc n))               â‰¡âŸ¨ length-++ (eâ„• n) âŸ©
  length (eâ„• n) + length [ suc n ]  â‰¡âŸ¨ cong (_+ 1) (eâ„•-length n) âŸ©
  suc n + 1                         â‰¡âŸ¨ cong suc (+-comm n 1) âŸ©
  suc (suc n)                       âˆ

EnumÃ— : Enum A â†’ Enum B â†’ Enum (A Ã— B)
EnumÃ— {A} {B} (mkEnum f f-cum f-wit) (mkEnum g g-cum g-wit) = mkEnum h h-cum h-wit where
  h : ğ•ƒâ‚™ (A Ã— B)
  h zero = f 0 [Ã—] g 0
  h (suc n) = h n ++ f n [Ã—] g n
  h-cum : Cumulation h
  h-cum n = f n [Ã—] g n , refl
  h-wit : âˆ€ xy â†’ h witness xy
  h-wit (x , y) = ğŸ™.map2 H (f-wit x) (g-wit y) where
    H : Witness f x â†’ Witness g y â†’ Witness h (x , y)
    H (m , xâˆˆfm) (n , xâˆˆgn) = suc (m + n) , âˆˆ-++âºÊ³ H2 where
      H2 : (x , y) âˆˆ f (m + n) [Ã—] g (m + n)
      H2 = âˆˆ[Ã—]-intro (cum-â‰¤â†’âŠ† f-cum mâ‰¤m+n xâˆˆfm) (cum-â‰¤â†’âŠ† g-cum mâ‰¤n+m xâˆˆgn)

instance
  Enum2â„• : Enum (â„• Ã— â„•)
  Enum2â„• = EnumÃ— Enumâ„• Enumâ„•

âˆˆe2â„•-intro : âˆ€ m n â†’ (m , n) âˆˆ enum (suc (m + n))
âˆˆe2â„•-intro m n = âˆˆ-++âºÊ³ $ âˆˆ[Ã—]-intro mâˆˆeâ„•m+n nâˆˆeâ„•m+n where
  mâˆˆeâ„•m+n : m âˆˆ eâ„• (m + n)
  mâˆˆeâ„•m+n = âˆˆeâ„•-intro m (m + n) mâ‰¤m+n
  nâˆˆeâ„•m+n : n âˆˆ eâ„• (m + n)
  nâˆˆeâ„•m+n = âˆˆeâ„•-intro n (m + n) mâ‰¤n+m

e2â„•-length-zero : length (enum zero) â‰¡ suc zero
e2â„•-length-zero = refl

e2â„•-length-suc : âˆ€ n â†’ length (enum (suc n)) â‰¡ length (enum n) + suc n * suc n
e2â„•-length-suc n =
  length (enum (suc n))                           â‰¡âŸ¨ length-++ (enum n) âŸ©
  length (enum n) + length (eâ„• n [Ã—] eâ„• n)        â‰¡âŸ¨ cong (length (enum n) +_) $ [Ã—]-length (eâ„• n) (eâ„• n) âŸ©
  length (enum n) + length (eâ„• n) * length (eâ„• n) â‰¡âŸ¨ cong (length (enum n) +_) $ cong2 _*_ (eâ„•-length n) (eâ„•-length n) âŸ©
  length (enum n) + suc n * suc n                 âˆ

e2â„•-length->n : âˆ€ n â†’ length (enum n) > n
e2â„•-length->n zero = â‰¤-refl
e2â„•-length->n (suc n) = subst (_> suc n) (e2â„•-length-suc n) H where
  H : length (enum n) + suc n * suc n > suc n
  H = +-mono-â‰¤ H2 (mâ‰¤m*n _ _) where
    H2 : 1 â‰¤ length (enum n)
    H2 = â‰¤-trans (sâ‰¤s zâ‰¤n) (e2â„•-length->n n)

e2â„•â“‚ : â„• â†’ (â„• Ã— â„•) ï¼Ÿ
e2â„•â“‚ n = enum n [ n ]?

e2â„•â“‚-enum : âˆ€ p â†’ Î£ k ï¼Œ e2â„•â“‚ k â‰¡ some p
e2â„•â“‚-enum (m , n) with enum (suc (m + n)) [ m , n ]â»Â¹? in eq1
... | none rewrite xâˆˆâ†’Î£[x]â»Â¹? (âˆˆe2â„•-intro m n) .snd with eq1
... | ()
e2â„•â“‚-enum (m , n) | some k with e2â„•â“‚ k in eq2
... | none rewrite Î£[<length]? (Enum2â„• .enum k) (e2â„•-length->n k) .snd with eq2
... | ()
e2â„•â“‚-enum (m , n) | some k | some q = k , H where
  --eq1 : e2â„• (suc (m + n)) [ m , n ]â»Â¹? â‰¡ some k
  --eq2 : e2â„•â“‚ k â‰¡ e2â„• k [ k ]? â‰¡ some q
  H : e2â„•â“‚ k â‰¡ some (m , n)
  H with â‰¤-total k (suc (m + n))
  ... | injâ‚ â‰¤ with cum-â‰¤â†’++ cum â‰¤
  ... | xs , eq3 =
    e2â„•â“‚ k                            â‰¡âŸ¨ eq2 âŸ©
    some q                            â‰¡Ë˜âŸ¨ ++[]? (enum k) eq2 âŸ©
    (enum k ++ xs) [ k ]?             â‰¡Ë˜âŸ¨ cong (_[ k ]?) eq3 âŸ©
    enum (suc (m + n)) [ k ]?         â‰¡âŸ¨ index-inv (enum (suc (m + n))) eq1 âŸ©
    some (m , n)                      âˆ
  H | injâ‚‚ â‰¥ with cum-â‰¤â†’++ cum â‰¥
  ... | xs , eq3 =
    e2â„•â“‚ k                            â‰¡âŸ¨ cong (_[ k ]?) eq3 âŸ©
    (enum (suc (m + n)) ++ xs) [ k ]? â‰¡âŸ¨ ++[]? (enum (suc (m + n))) (index-inv (enum (suc (m + n))) eq1) âŸ©
    some (m , n)                      âˆ

Enumâ“‚2â„• : â“‚.Enum (â„• Ã— â„•)
Enumâ“‚2â„• = e2â„•â“‚ , âˆ£_âˆ£â‚ âˆ˜ e2â„•â“‚-enum

Enumâ„™â†’â“‚ : {P : A â†’ ğ•‹ â„“} â†’ Enumâ„™ P â†’ â“‚.Enumâ„™ P
Enumâ„™â†’â“‚ {A} {P} (mkEnumâ„™ f f-cum f-wit) = g , g-wit where
  g : â„• â†’ A ï¼Ÿ
  g n with e2â„•â“‚ n
  ... | some (m , n) = f m [ n ]?
  ... | none = none
  g-cal : âˆ€ k {m n} â†’ e2â„•â“‚ k â‰¡ some (m , n) â†’ g k â‰¡ f m [ n ]?
  g-cal _ eq rewrite eq = refl
  g-wit : âˆ€ x â†’ P x â†” g â“‚.witness x
  g-wit x = â†”-trans (f-wit x) $ â‡’: ğŸ™.map (uncurry H1) â‡: ğŸ™.map (uncurry H2) where
    H1 : âˆ€ n â†’ x âˆˆ f n â†’ â“‚.Witness g x
    H1 m xâˆˆfn with âˆˆâ†’Î£[]? xâˆˆfn
    ... | n , fm[n] with e2â„•â“‚-enum (m , n)
    ... | k , eq = k , g-cal k eq âˆ™ fm[n]
    H2 : âˆ€ n â†’ g n â‰¡ some x â†’ Witness f x
    H2 k fm[n] with e2â„•â“‚ k
    ... | some (m , n) with []?â†’âˆˆ (f m) fm[n]
    ... | xâˆˆfm = m , xâˆˆfm

Enumâ„™â†â“‚ : {P : A â†’ ğ•‹ â„“} â†’ â“‚.Enumâ„™ P â†’ Enumâ„™ P
Enumâ„™â†â“‚ {A} {P} (f , f-enum) = mkEnumâ„™ h h-cum h-enum where
  g : ğ•ƒâ‚™ A
  g n with f n
  ... | some x = [ x ]
  ... | none = []
  g-cal : âˆ€ {k x} â†’ f k â‰¡ some x â†’ g k â‰¡ [ x ]
  g-cal eq rewrite eq = refl
  witâ†” : âˆ€ x â†’ â“‚.Witness f x â†” Witness g x
  witâ†” x = â‡’: uncurry H1 â‡: uncurry H2 where
    H1 : âˆ€ n â†’ f n â‰¡ some x â†’ Witness g x
    H1 n fn = n , subst (x âˆˆ_) (g-cal fn) (here refl)
    H2 : âˆ€ n â†’ x âˆˆ g n â†’ â“‚.Witness f x
    H2 n xâˆˆgn with f n in eq
    H2 n (here refl) | some x = n , eq
  h : ğ•ƒâ‚™ A
  h zero = []
  h (suc n) = h n ++ g n
  h-cum : Cumulation h
  h-cum n = g n , refl
  h-enum : âˆ€ x â†’ P x â†” h witness x
  h-enum x =
    P x           â†”âŸ¨ f-enum x âŸ©
    f â“‚.witness x â†”âŸ¨ â†”-map $ witâ†” x âŸ©
    g witness x   â†”âŸ¨ â†”-map $ â‡’: uncurry H1 â‡: uncurry H2 âŸ©
    h witness x   â†”âˆ where
      H1 : âˆ€ n â†’ x âˆˆ g n â†’ Witness h x
      H1 n xâˆˆgn = suc n , âˆˆ-++âºÊ³ xâˆˆgn
      H2 : âˆ€ n â†’ x âˆˆ h n â†’ Witness g x
      H2 (suc n) xâˆˆhn++gn with âˆˆ-++â» (h n) xâˆˆhn++gn
      ... | injâ‚ xâˆˆhn = H2 n xâˆˆhn
      ... | injâ‚‚ xâˆˆgn = n , xâˆˆgn

Enumâ„™â†”â“‚ : Enumâ„™ P â†” â“‚.Enumâ„™ P
Enumâ„™â†”â“‚ = â‡’: Enumâ„™â†’â“‚ â‡: Enumâ„™â†â“‚

Enumâ†”â“‚ : Enum A â†” â“‚.Enum A
Enumâ†”â“‚ {A} =
  Enum A                  â†”âŸ¨ Enumâ†”â„™ âŸ©
  Enumâ„™ (Î» (_ : A) â†’ âŠ¤)   â†”âŸ¨ Enumâ„™â†”â“‚ âŸ©
  â“‚.Enumâ„™ (Î» (_ : A) â†’ âŠ¤) â†”Ë˜âŸ¨ â“‚.Enumâ†”â„™ âŸ©
  â“‚.Enum A                â†”âˆ

enumerableâ„™â†”â“‚ : enumerableâ„™ P â†” â“‚.enumerableâ„™ P
enumerableâ„™â†”â“‚ = â†”-map Enumâ„™â†”â“‚

enumerableâ†”â“‚ : enumerable A â†” â“‚.enumerable A
enumerableâ†”â“‚ {A} = â†”-map Enumâ†”â“‚

discrâ†’enumâ†’count : discrete A â†’ enumerable A â†’ countable A
discrâ†’enumâ†’count disA enumA =
  â“‚.discrâ†’enumâ†’count disA (enumerableâ†”â“‚ .â‡’ enumA)
